Use an EEnvMap in OptimizePropDiscr for more efficient lookups

erasure/theories/EEnvMap.v
@@ -1,7 +1,11 @@
 From Coq Require Import ssreflect ssrbool.
+From Equations Require Import Equations.
 From MetaCoq.Template Require Import utils Kernames EnvMap.
 From MetaCoq.Erasure Require Import EAst EGlobalEnv EAstUtils EGlobalEnv EAstUtils.
 Import MCMonadNotation.
+
+Lemma fresh_globals_cons_inv {Σ : global_context} {d} : EnvMap.fresh_globals (d :: Σ) -> EnvMap.fresh_globals Σ.
+Proof. intros H; now depelim H. Qed.
 
 Module GlobalContextMap.
   Record t := 
@@ -9,19 +13,39 @@ Module GlobalContextMap.
     map : EnvMap.t global_decl;
     repr : EnvMap.repr global_decls map;
     wf : EnvMap.fresh_globals global_decls }.
-  
+
+  Definition lookup_env Σ kn := EnvMap.lookup kn Σ.(map).
+
+  Lemma lookup_env_spec (Σ : t) kn : lookup_env Σ kn = EGlobalEnv.lookup_env Σ kn.
+  Proof. 
+    rewrite /lookup_env.
+    rewrite (EnvMap.lookup_spec Σ.(global_decls)) //; apply Σ.
+  Qed.
+
   Definition lookup_minductive Σ kn : option mutual_inductive_body :=
-    decl <- EnvMap.lookup kn Σ.(map);; 
+    decl <- lookup_env Σ kn;; 
     match decl with
     | ConstantDecl _ => None
     | InductiveDecl mdecl => ret mdecl
     end.
+
+  Lemma lookup_minductive_spec Σ kn : lookup_minductive Σ kn = EGlobalEnv.lookup_minductive Σ kn.
+  Proof.
+    rewrite /lookup_minductive /EGlobalEnv.lookup_minductive.
+    rewrite lookup_env_spec //.
+  Qed.
 
   Definition lookup_inductive Σ kn : option (mutual_inductive_body * one_inductive_body) :=
     mdecl <- lookup_minductive Σ (inductive_mind kn) ;;
     idecl <- nth_error mdecl.(ind_bodies) (inductive_ind kn) ;;
     ret (mdecl, idecl).
   
+  Lemma lookup_inductive_spec Σ kn : lookup_inductive Σ kn = EGlobalEnv.lookup_inductive Σ kn.
+  Proof.
+    rewrite /lookup_inductive /EGlobalEnv.lookup_inductive.
+    rewrite lookup_minductive_spec //.
+  Qed.
+    
   Definition lookup_inductive_pars Σ kn : option nat := 
     mdecl <- lookup_minductive Σ kn ;;
     ret mdecl.(ind_npars).
@@ -29,10 +53,18 @@ Module GlobalContextMap.
   Lemma lookup_inductive_pars_spec Σ kn : lookup_inductive_pars Σ kn = EGlobalEnv.lookup_inductive_pars Σ kn.
   Proof.
     rewrite /lookup_inductive_pars /EGlobalEnv.lookup_inductive_pars.
-    rewrite /lookup_inductive /EGlobalEnv.lookup_inductive.
-    rewrite /lookup_minductive /EGlobalEnv.lookup_minductive.
-    rewrite (EnvMap.lookup_spec Σ.(global_decls)).
-    eapply wf. eapply repr. reflexivity.
+    now rewrite lookup_minductive_spec.
+  Qed.
+
+  Definition inductive_isprop_and_pars Σ (ind : inductive) :=
+    '(mdecl, idecl) <- lookup_inductive Σ ind ;;
+    ret (ind_propositional idecl, ind_npars mdecl).
+  
+  Lemma inductive_isprop_and_pars_spec Σ kn : 
+    inductive_isprop_and_pars Σ kn = EGlobalEnv.inductive_isprop_and_pars Σ kn.
+  Proof.
+    rewrite /inductive_isprop_and_pars /EGlobalEnv.inductive_isprop_and_pars.
+    now rewrite lookup_inductive_spec.
   Qed.
 
   Program Definition make (g : global_declarations) (Hg : EnvMap.fresh_globals g): t :=
