erasure/theories/EProgram.v
@@ -4,8 +4,8 @@ From Equations Require Import Equations.
 From MetaCoq.Template Require Import Transform bytestring config utils BasicAst.
 From MetaCoq.PCUIC Require PCUICAst PCUICAstUtils PCUICProgram.
 From MetaCoq.SafeChecker Require Import PCUICErrors PCUICWfEnvImpl.
-From MetaCoq.Erasure Require EAstUtils ErasureFunction ErasureCorrectness EPretty Extract.
-From MetaCoq.Erasure Require ErasureFunction EWellformed EEtaExpanded EWcbvEval EDeps.
+From MetaCoq.Erasure Require EAstUtils EPretty.
+From MetaCoq.Erasure Require EWellformed EEnvMap EWcbvEval EDeps.
 
 Import bytestring.
 Local Open Scope bs.
@@ -30,7 +30,7 @@ Definition eprogram_env := (EEnvMap.GlobalContextMap.t * EAst.term).
 
 Import EEnvMap.GlobalContextMap (make, global_decls).
 
-Arguments EWcbvEval.eval {wfl} _ _ _.
+Global Arguments EWcbvEval.eval {wfl} _ _ _.
 
 Definition wf_eprogram (efl : EEnvFlags) (p : eprogram) :=
   @wf_glob efl p.1 /\ @wellformed efl p.1 0 p.2.
@@ -59,69 +59,3 @@ Proof.
   intros wf; depelim wf. constructor; auto.
 Qed.
   
-Program Definition erase_pcuic_program (p : pcuic_program) 
-  (wfΣ : ∥ PCUICTyping.wf_ext (H := config.extraction_checker_flags) p.1 ∥)
-  (wt : ∥ ∑ T, PCUICTyping.typing (H := config.extraction_checker_flags) p.1 [] p.2 T ∥) : eprogram_env :=
-  let wfe := build_wf_env_from_env p.1.1 (map_squash (PCUICTyping.wf_ext_wf _) wfΣ) in
-  let wfe' := ErasureFunction.make_wf_env_ext wfe p.1.2 wfΣ in
-  let t := ErasureFunction.erase wfe' nil p.2 _ in
-  let Σ' := ErasureFunction.erase_global (EAstUtils.term_global_deps t) wfe in
-  (EEnvMap.GlobalContextMap.make Σ' _, t).
-  
-Next Obligation.
-  sq. destruct wt as [T Ht].
-  cbn in *. subst. now exists T.
-Qed.
-Next Obligation.
-  unfold ErasureFunction.erase_global.
-  eapply wf_glob_fresh.
-  eapply ErasureFunction.erase_global_decls_wf_glob.
-Qed.
-
-Obligation Tactic := idtac.
-
-Import Extract.
-
-Definition expanded_eprogram (p : eprogram) := 
-  EEtaExpandedFix.isEtaExp_env p.1 && EEtaExpandedFix.isEtaExp p.1 [] p.2.
-
-Definition expanded_eprogram_env (p : eprogram_env) := 
-  let decls := p.1.(EEnvMap.GlobalContextMap.global_decls) in
-  EEtaExpandedFix.isEtaExp_env decls && EEtaExpandedFix.isEtaExp decls [] p.2.
-
-Definition expanded_eprogram_cstrs (p : eprogram) := 
-  EEtaExpanded.isEtaExp_env p.1 && EEtaExpanded.isEtaExp p.1 p.2.
-
-Definition expanded_eprogram_env_cstrs (p : eprogram_env) := 
-  let decls := p.1.(EEnvMap.GlobalContextMap.global_decls) in
-  EEtaExpanded.isEtaExp_env decls && EEtaExpanded.isEtaExp decls p.2.
-  
-Definition erase_program (p : pcuic_program) (wtp : ∥ wt_pcuic_program (cf:=config.extraction_checker_flags) p ∥) : eprogram_env :=
-  erase_pcuic_program p (map_squash fst wtp) (map_squash snd wtp).
-
-Lemma expanded_erase_program (cf := config.extraction_checker_flags) p (wtp : ∥ wt_pcuic_program p ∥) :
-  PCUICEtaExpand.expanded_pcuic_program p ->
-  expanded_eprogram_env (erase_program p wtp).
-Proof.
-  intros [etaenv etat]. apply /andP; split.
-  eapply EEtaExpandedFix.expanded_global_env_isEtaExp_env, ErasureFunction.expanded_erase_global, etaenv.
-  eapply EEtaExpandedFix.expanded_isEtaExp, ErasureFunction.expanded_erase, etat.
-Qed.
-
-Lemma expanded_eprogram_env_expanded_eprogram_cstrs p :
-  expanded_eprogram_env p ->
-  expanded_eprogram_env_cstrs p.
-Proof.
-  move=> /andP[] etaenv etat.
-  apply /andP. split; [now eapply EEtaExpanded.isEtaExpFix_env_isEtaExp_env|
-  now eapply EEtaExpanded.isEtaExpFix_isEtaExp].
-Qed.
-
-Lemma expanded_eprogram_expanded_eprogram_cstrs p :
-  expanded_eprogram p ->
-  expanded_eprogram_cstrs p.
-Proof.
-  move=> /andP[] etaenv etat.
-  apply /andP. split; [now eapply EEtaExpanded.isEtaExpFix_env_isEtaExp_env|
-  now eapply EEtaExpanded.isEtaExpFix_isEtaExp].
-Qed.
