erasure/theories/ETransform.v
@@ -13,13 +13,69 @@ Import PCUICAst (term) PCUICProgram PCUICTransform (eval_pcuic_program) Extract 
     EAst Transform ERemoveParams.
 Import EEnvMap EGlobalEnv EWellformed.
 
+Program Definition erase_pcuic_program (p : pcuic_program) 
+  (wfΣ : ∥ PCUICTyping.wf_ext (H := config.extraction_checker_flags) p.1 ∥)
+  (wt : ∥ ∑ T, PCUICTyping.typing (H := config.extraction_checker_flags) p.1 [] p.2 T ∥) : eprogram_env :=
+  let wfe := build_wf_env_from_env p.1.1 (map_squash (PCUICTyping.wf_ext_wf _) wfΣ) in
+  let wfe' := ErasureFunction.make_wf_env_ext wfe p.1.2 wfΣ in
+  let t := ErasureFunction.erase wfe' nil p.2 _ in
+  let Σ' := ErasureFunction.erase_global (EAstUtils.term_global_deps t) wfe in
+  (EEnvMap.GlobalContextMap.make Σ' _, t).
+  
+Next Obligation.
+  sq. destruct wt as [T Ht].
+  cbn in *. subst. now exists T.
+Qed.
+Next Obligation.
+  unfold ErasureFunction.erase_global.
+  eapply wf_glob_fresh.
+  eapply ErasureFunction.erase_global_decls_wf_glob.
+Qed.
+
+Obligation Tactic := idtac.
+
+Import Extract.
+  
+Definition erase_program (p : pcuic_program) (wtp : ∥ wt_pcuic_program (cf:=config.extraction_checker_flags) p ∥) : eprogram_env :=
+  erase_pcuic_program p (map_squash fst wtp) (map_squash snd wtp).
+
+Lemma expanded_erase_program (cf := config.extraction_checker_flags) p (wtp : ∥ wt_pcuic_program p ∥) :
+  PCUICEtaExpand.expanded_pcuic_program p ->
+  EEtaExpandedFix.expanded_eprogram_env (erase_program p wtp).
+Proof.
+  intros [etaenv etat]. split.
+  eapply ErasureFunction.expanded_erase_global, etaenv.
+  eapply ErasureFunction.expanded_erase, etat.
+Qed.
+
+Lemma expanded_eprogram_env_expanded_eprogram_cstrs p :
+  EEtaExpandedFix.expanded_eprogram_env p ->
+  EEtaExpanded.expanded_eprogram_env_cstrs p.
+Proof.
+  move=> [] etaenv etat.
+  apply /andP.
+  split.
+  - eapply EEtaExpanded.isEtaExpFix_env_isEtaExp_env. now eapply EEtaExpandedFix.expanded_global_env_isEtaExp_env.
+  - eapply EEtaExpanded.isEtaExpFix_isEtaExp. now eapply EEtaExpandedFix.expanded_isEtaExp.
+Qed.
+
+(* Lemma expanded_eprogram_expanded_eprogram_cstrs p :
+  expanded_eprogram p ->
+  expanded_eprogram_cstrs p.
+Proof.
+  move=> /andP[] etaenv etat.
+  apply /andP. split; [now eapply EEtaExpanded.isEtaExpFix_env_isEtaExp_env|
+  now eapply EEtaExpanded.isEtaExpFix_isEtaExp].
+Qed. *)
+
+
 Program Definition erase_transform : Transform.t pcuic_program eprogram_env PCUICAst.term EAst.term 
   eval_pcuic_program (eval_eprogram_env EWcbvEval.default_wcbv_flags) :=
  {| name := "erasure";
     pre p :=  
       ∥ wt_pcuic_program (cf := config.extraction_checker_flags) p ∥ /\ PCUICEtaExpand.expanded_pcuic_program p ;
     transform p hp := erase_program p (proj1 hp) ;
-    post p := [/\ wf_eprogram_env all_env_flags p & expanded_eprogram_env p];
+    post p := [/\ wf_eprogram_env all_env_flags p & EEtaExpandedFix.expanded_eprogram_env p];
     obseq g g' v v' := let Σ := g.1 in Σ ;;; [] |- v ⇝ℇ v' |}.
 Next Obligation.
   cbn -[erase_program].
@@ -58,16 +114,35 @@ Program Definition guarded_to_unguarded_fix {fl : EWcbvEval.WcbvFlags} {efl : EE
     (eval_eprogram_env fl) (eval_eprogram_env (EEtaExpandedFix.switch_unguarded_fix fl)) :=
   {| name := "switching to unguarded fixpoints";
     transform p pre := p;
-    pre p := wf_eprogram_env efl p /\ expanded_eprogram_env p;
-    post p := wf_eprogram_env efl p /\ expanded_eprogram_env p;
+    pre p := wf_eprogram_env efl p /\ EEtaExpandedFix.expanded_eprogram_env p;
+    post p := wf_eprogram_env efl p /\ EEtaExpandedFix.expanded_eprogram_env p;
     obseq g g' v v' := v' = v |}.
 Next Obligation. cbn. eauto. Qed.
 Next Obligation.
   cbn.
-  move=> fl efl wguard [Σ t] v [wfp /andP[etae etat]]. cbn in *.
+  move=> fl efl wguard [Σ t] v [wfp [etae etat]]. cbn in *.
   intros [ev]. exists v. split => //.
   red. sq. cbn in *.
-  apply EEtaExpandedFix.eval_opt_to_target => //. apply wfp.
+  apply EEtaExpandedFix.eval_opt_to_target => //. 2:apply wfp.
+  now eapply EEtaExpandedFix.expanded_global_env_isEtaExp_env.
+  now eapply EEtaExpandedFix.expanded_isEtaExp.
+Qed.
+
+Definition rebuild_wf_env {efl} (p : eprogram) (hwf : wf_eprogram efl p): eprogram_env :=
+  (GlobalContextMap.make p.1 (wf_glob_fresh p.1 (proj1 hwf)), p.2).
+
+Program Definition rebuild_wf_env_transform {fl : EWcbvEval.WcbvFlags} {efl} : 
+  Transform.t eprogram eprogram_env EAst.term EAst.term (eval_eprogram fl) (eval_eprogram_env fl) :=
+  {| name := "rebuilding environment lookup table";
+     pre p := wf_eprogram efl p /\ EEtaExpanded.expanded_eprogram_cstrs p;
+     transform p pre := rebuild_wf_env p (proj1 pre);
+     post p := wf_eprogram_env efl p /\ EEtaExpanded.expanded_eprogram_env_cstrs p;
+     obseq g g' v v' := v = v' |}.
+Next Obligation.
+  cbn. intros fl efl input [wf exp]. cbn; split => //.
+Qed.
+Next Obligation.
+  cbn. intros fl efl input v [] ev p'; exists v. split => //.
 Qed.
 
 Program Definition remove_params_optimization {fl : EWcbvEval.WcbvFlags} 
@@ -75,8 +150,8 @@ Program Definition remove_params_optimization {fl : EWcbvEval.WcbvFlags}
   Transform.t eprogram_env eprogram EAst.term EAst.term (eval_eprogram_env fl) (eval_eprogram fl) :=
   {| name := "stripping constructor parameters";
     transform p pre := ERemoveParams.strip_program p;
-    pre p := wf_eprogram_env efl p /\ expanded_eprogram_env_cstrs p;
-    post p := wf_eprogram (switch_no_params efl) p /\ expanded_eprogram_cstrs p;
+    pre p := wf_eprogram_env efl p /\ EEtaExpanded.expanded_eprogram_env_cstrs p;
+    post p := wf_eprogram (switch_no_params efl) p /\ EEtaExpanded.expanded_eprogram_cstrs p;
     obseq g g' v v' := v' = (ERemoveParams.strip g.1 v) |}.
 Next Obligation.
   move=> fl efl [Σ t] [wfp etap].
@@ -101,8 +176,8 @@ Program Definition remove_params_fast_optimization (fl : EWcbvEval.WcbvFlags)
   Transform.t eprogram_env eprogram EAst.term EAst.term (eval_eprogram_env fl) (eval_eprogram fl) :=
   {| name := "stripping constructor parameters (faster?)";
     transform p _ := (ERemoveParams.Fast.strip_env p.1, ERemoveParams.Fast.strip p.1 [] p.2);
-    pre p := wf_eprogram_env efl p /\ expanded_eprogram_env_cstrs p;
-    post p := wf_eprogram (switch_no_params efl) p /\ expanded_eprogram_cstrs p;
+    pre p := wf_eprogram_env efl p /\ EEtaExpanded.expanded_eprogram_env_cstrs p;
+    post p := wf_eprogram (switch_no_params efl) p /\ EEtaExpanded.expanded_eprogram_cstrs p;
     obseq g g' v v' := v' = (ERemoveParams.strip g.1 v) |}.
 Next Obligation.
   move=> fl efl [Σ t] [wfp etap].
@@ -129,11 +204,11 @@ Qed.
 Import EOptimizePropDiscr EWcbvEval.
 
 Program Definition optimize_prop_discr_optimization {fl : WcbvFlags} {efl : EEnvFlags} {hastrel : has_tRel} {hastbox : has_tBox} :
-  self_transform eprogram EAst.term (eval_eprogram fl) (eval_eprogram (disable_prop_cases fl)) := 
+  Transform.t eprogram_env eprogram EAst.term EAst.term (eval_eprogram_env fl) (eval_eprogram (disable_prop_cases fl)) := 
   {| name := "optimize_prop_discr"; 
     transform p _ := optimize_program p ; 
-    pre p := wf_eprogram efl p /\ expanded_eprogram_cstrs p;
-    post p := wf_eprogram efl p /\ expanded_eprogram_cstrs p;
+    pre p := wf_eprogram_env efl p /\ EEtaExpanded.expanded_eprogram_env_cstrs p;
+    post p := wf_eprogram efl p /\ EEtaExpanded.expanded_eprogram_cstrs p;
     obseq g g' v v' := v' = EOptimizePropDiscr.optimize g.1 v |}.
 
 Next Obligation.
